Created: 2024-10-23 18:01
Category: #automata-theory 
Status: #philnits



# 2016S_FE_AM_6 %% ex. 2024S_FE-A_83 %%

There is a language defined by a context-free grammar with the production rules below:
E -> T + E | T
T -> F * T | F
F -> ( E ) | C
C -> 0 | 1 | 2 | 3 | 4 | 5 | 6 | 7 | 8 | 9

In this grammar, non-terminals are E, T, F, and C; terminals are parentheses, plus sign, asterisk, and numbers; E is the start symbol. Which of the following shows that the expression 7 + 3 * (6 + 4) is a sentence of this language?

a) E -> 7 + 3 * (F + T) 
b) E -> 7 + 3 * E 
c) E -> 7 + 3 * (T) 
d) E -> 7 + T * (E)
? 
d) E -> 7 + T * (E)

### Why E → 7 + 3 * (F + T) works:

1. First, verify this specific sequence can generate our target "7 + 3 * (6 + 4)":
    - 7 is already there
    - 3 is already there
    - F can derive a single digit (F → C → 6)
    - T can derive a single digit (T → F → C → 4)
2. The other options fail because: b) E → 7 + 3 * E
    
    - Can't generate the parentheses pattern at all
    
    c) E → 7 + 3 * (T)
    
    - Has parentheses but can't generate "number + number" inside them
    - Only has T inside, not a sum
    
    d) E → 7 + T * (E)
    - Has the wrong constant (T instead of 3)
    - Wrong order of operations

We need to verify that:

1. The constants match exactly where needed (7 and 3)
2. The structure matches (* and + in correct positions)
3. The non-terminals (F and T) can actually derive what we need
4. The parentheses are in the right place



%% ignore this %%
---









# References %% add your references here %%
- 